```
zeta(s, z)
```

Generalized zeta function defined by

$$
\zeta(s, z) = \sum_{k=0}^\infty \frac{1}{((k+z)^2)^{s/2}},
$$

where any term with $k+z = 0$ is excluded.  For $\Re(z) > 0$, this definition is equivalent to the Hurwitz zeta function $\sum_{k=0}^\infty (k+z)^{-s}$.

The Riemann zeta function is recovered as $\zeta(s) = \zeta(s,1)$.

External links: [Riemann zeta function](https://en.wikipedia.org/wiki/Riemann_zeta_function), [Hurwitz zeta function](https://en.wikipedia.org/wiki/Hurwitz_zeta_function)
